Bank_SN_Proofs.v
@@ -20,11 +20,11 @@ Section Bank_SN_Proofs.
   Theorem transformed_min_value_invariant :
     forall (net : bank_sn_network) tr,
       step_dup_star (params := bank_sn_multi_params) step_async_init net tr ->
-      min_value_invariant_net (revertNetwork net).
+      min_value_invariant_network (revertNetwork net).
   Proof using.
     intros.
     pose proof @true_in_reachable_transform _ bank_multi_params 
-               (fun net : network => min_value_invariant_net net)
+               (fun net : network => min_value_invariant_network net)
                true_in_reachable_min_value.
     unfold true_in_reachable in *.
     apply H0. unfold reachable. eauto.
