Bank_Utils.v
@@ -1,0 +1,150 @@
+Require Import Bank.
+
+From Verdi Require Import
+  Verdi
+  HandlerMonad
+  LabeledNet.
+
+From InfSeqExt Require Import
+  infseq
+  classical.
+
+Local Arguments update {_} {_} _ _ _ _ _ : simpl never.
+
+Set Bullet Behavior "Strict Subproofs".
+
+
+Lemma In_split_not_In :
+  forall A (p : A) p' xs ys zs,
+    In p (xs ++ p' :: ys) ->
+    ~ In p (zs ++ xs ++ ys) ->
+    p = p'.
+Proof using.
+  intros. find_apply_lem_hyp in_app_iff. simpl in *.
+  intuition ; find_false ; apply in_app_iff
+            ; right ; apply in_app_iff ; auto.
+Qed.
+
+Lemma option_eq_dec : forall {T : Type} (T_eq_dec : forall t1 t2 : T, {t1 = t2} + {t1 <> t2}),
+  forall l1 l2 : option T, {l1 = l2} + {l1 <> l2}.
+Proof.
+  repeat decide equality.
+Qed.
+
+
+Definition label_eq_dec :
+  forall x y : label,
+    {x = y} + {x <> y}.
+Proof using.
+  decide equality; apply fin_eq_dec.
+Qed.
+
+
+Ltac basic_unfold :=
+  repeat ( unfold step_async_init,
+                  unlabeled_input_handlers, unlabeled_net_handlers,
+                  lb_net_handlers, lb_input_handlers,
+                  net_handlers, input_handlers in *
+         ; repeat break_let
+         ).
+
+Ltac simplify_bank_handlers :=
+  repeat ( monad_unfold
+         ; basic_unfold
+         ; unfold InitState,
+                  NetHandler, AgentNetHandler, ServerNetHandler,
+                  IOHandler,  AgentIOHandler,  ServerIOHandler in *
+         ; repeat break_match ; simpl in * )
+  ; try solve_by_inversion
+  ; repeat ( repeat (find_inversion ; intuition)
+           ; subst_max ; simpl in * ; intuition )
+  ; repeat clean.
+
+
+Definition initialized_network (net:network) :=
+  exists tr, step_async_star step_async_init net tr.
+
+Definition initialized_eventseq (s:infseq (event network label (name * (input + list output)))) :=
+  event_step_star step_async step_async_init (hd s).
+
+
+Lemma step_star_consistent_state :
+  forall net,
+    initialized_network net ->
+    (exists astate, nwState net Agent = agent astate) /\
+    (exists sstate, nwState net Server = server sstate) /\
+    (forall sstate, nwState net Agent <> server sstate) /\
+    (forall astate, nwState net Server <> agent astate).
+Proof using.
+  intros net Hstar. unfold initialized_network in *. break_exists_name tr.
+  find_apply_lem_hyp refl_trans_1n_n1_trace.
+  prep_induction Hstar. induction Hstar.
+  - intuition ; break_exists ; subst_max ; simplify_bank_handlers ; eauto.
+  - intuition ; subst_max ; invcs H0 ; simplify_bank_handlers
+                ; unfold update ; simpl ; eauto
+                ; repeat break_exists ; unfold update in * ; simpl in * ; discriminate.
+Qed.
+
+Definition message_enables_label p l :=
+  forall net,
+    initialized_network net ->
+    In p (nwPackets net) ->
+    lb_step_ex lb_step_async l net.
+
+Definition message_delivered_label p l :=
+  forall l' net net' tr,
+    initialized_network net ->
+    lb_step_async net l' net' tr ->
+    In p (nwPackets net) ->
+    ~ In p (nwPackets net') ->
+    l = l'.
+
+Lemma messages_trigger_labels :
+  forall l p,
+    message_enables_label p l ->
+    message_delivered_label p l ->
+    forall s,
+      initialized_eventseq s ->
+      lb_step_execution lb_step_async s ->
+      In p (nwPackets (evt_a (hd s))) ->
+      weak_until (now (enabled lb_step_async l))
+                 (now (occurred l))
+                 s.
+Proof using.
+    intros l p Henables Hdelivered. unfold initialized_eventseq.
+    cofix c. destruct s, e.
+    intros Hstar Hexec Hin. invcs Hexec.
+    destruct (label_eq_dec l evt_l) ; subst_max.
+    - apply W0. easy.
+    - apply W_tl ; simpl.
+      + unfold message_enables_label, initialized_network in *.
+        unfold enabled. simpl. now eauto.
+      + apply c ; simpl ; intuition.
+        * unfold event_step_star in *. unfold bank_multi_params. rewrite H2.
+          apply (step_async_star_lb_step_reachable Hstar H1).
+        * destruct (In_dec packet_eq_dec
+                         p (nwPackets (LabeledNet.evt_a e'))) ; intuition.
+          unfold message_delivered_label in *.
+Admitted.
+
+Lemma message_labels_eventually_occur :
+  forall l p,
+    l <> label_silent ->
+    message_enables_label p l ->
+    message_delivered_label p l ->
+    forall s,
+      initialized_eventseq s ->
+      weak_fairness lb_step_async label_silent s ->
+      lb_step_execution lb_step_async s ->
+      In p (nwPackets (evt_a (hd s))) ->
+      eventually (now (occurred l)) s.
+Proof using.
+    intros.
+    find_eapply_lem_hyp messages_trigger_labels ; eauto.
+    find_apply_lem_hyp weak_until_until_or_always.
+    intuition.
+    - now eauto using until_eventually.
+    - find_apply_lem_hyp always_continuously.
+      eapply_prop_hyp weak_fairness continuously; auto.
+      destruct s. now find_apply_lem_hyp always_now.
+Qed.
