Makefile
@@ -3,10 +3,12 @@ OCAML = ocamlbuild -package uuidm -package verdi-runtime -I ml
 OCAML_BUILD     = $(OCAML) -cflags -w,a
 OCAML_DBG_BUILD = $(OCAML) -cflags -g
 
+COQ       = coqc
+COQ_QUICK = $(COQ) -quick
 
 
 BANK_EXTRACT    = Bank.v Bank_Extract.v
-BANK_PROVE      = Bank.v Bank_Proofs.v
+BANK_PROVE      = Bank.v Bank_Utils.v Bank_Proofs.v
 BANK_SN_EXTRACT = Bank.v Bank_SN.v Bank_SN_Extract.v
 BANK_SN_PROVE   = $(BANK_PROVE) Bank_SN.v Bank_SN_Proofs.v
 
@@ -25,10 +27,10 @@ quick: $(BANK_SN_PROVE:.v=.vio)
 
 
 %.vio: %.v
-	coqc -quick $<
+	$(COQ_QUICK) $<
 
 %.vo: %.v
-	coqc $<
+	$(COQ) $<
 
 
 bank.bin: $(BANK)
